\documentclass{article}
\usepackage{amsmath}
\usepackage{bm}
\usepackage{lettrine}
\usepackage{multicol}
\usepackage{geometry}
\geometry{a4paper,scale=0.8}

\begin{document}
\begin{multicols}{2}

\section{EEG two-factor zhang wang}


SSA $SST=SSA+SSB+SSAB+SSE$, where $SSA$, $SSB$, $SSE$,


$SST=\sum\limits_{i=1}^{a}\sum\limits_{j=1}^{b}\sum\limits_{k=1}^{n}\left( y_{ijk}-\left\langle y\right\rangle \right) ^2$,


$SSA=bn\sum\limits_{i=1}^{a}(\bar{A}_i- \left\langle y\right\rangle  )^2$,


$SSB=an\sum\limits_{j=1}^{b}(\bar{B}_i- \left\langle y\right\rangle  )^2$,


$SSE=\sum\limits_{i=1}^{a}\sum\limits_{j=1}^{b}\sum\limits_{k=1}^{n}(y_{ijk}-\bar{y}_{ij})^2$,


$MSA=\frac{SSA}{a-1},MSB=\frac{SSB}{b-1},MSAB=\frac{SSAB}{(a-1)(b-1)},MSE=\frac{SSE}{ab(n-1)}$,


$F_A=\frac{MSA}{MSE},F_B=\frac{MSB}{MSE},F_{AB}=\frac{MSAB}{MSE}$,


$F>F_c$,


$F<F_c$,


$\bm{C}=COV(\bm{X_1,X_2})=\frac{\sum\limits_{i=1}^{i=n}\left( X_{1,i}-\bar{X}_1\right) \left( X_{2,i}-\bar{X}_2 \right)}{n-1} $,


$t=\frac{\bar{x}-\mu}{s/\sqrt{n}}$,


$t^2$,


$t^2=\frac{(\bar{x}-\mu)^2}{s^2/n}$,


$t^2=n(\bar{x}-\mu)\left( \frac{1}{s^2}\right) (\bar{x}-\mu)$,


$T^2=n(\bm{\bar{X}}-\mu)^T\bm{C}^{-1}(\bm{\bar{x}}-\mu)$,


$\bm{\bar{X}}$,


$\bm{C}^{-1}$,


$\bm{\mu}$,


$\bm{C_1}$,


$\bm{C_2}$,
















\begin{align}
SST=\sum_{i=1}^{a}\sum_{j=1}^{b}\sum_{k=1}^{n}\left( y_{ijk}-\left\langle y\right\rangle \right) ^2
\end{align}




\end{multicols}
\end{document}